I think this is a dead end, so I'm committing
Will manually undo my changes lol

DatalogSemantics.v
@@ -278,46 +278,55 @@ Module RelSemantics.
       end
     else None.
   
+  Definition tt_set_prod (v1 v2: tt_set.t) :=
+    list_prod (tt_set.elements v1) (tt_set.elements v2).
   
-    
-                  
   
-  Definition join_relations (jvs: list string) (v1 v2: ListSet.set tup_type) :=
-    set_fold_left (fun (acc: ListSet.set tup_type) (elmt: (tup_type * tup_type)) =>
+  
+  Definition join_relations (jvs: list string) (v1 v2: tt_set.t) :=
+    List.fold_left (fun (acc: tt_set.t) (elmt: (tup_type * tup_type)) =>
                            let (t1, t2) := elmt in
                            match join_tuples jvs t1 t2 with
-                           | Some tup => set_add str_gt_list_ot.eq_dec tup acc
+                           | Some tup => tt_set.add tup acc
                            | None => acc
                            end)
-                        (set_prod v1 v2)
-                        (@empty_set tup_type).
+                        (tt_set_prod v1 v2)
+                        (tt_set.empty).
 
-  Definition select_relation (n: string) (g: ground_types) (v: ListSet.set tup_type) :=
-    set_fold_left (fun (acc: ListSet.set tup_type) (elmt: tup_type) =>
-                     match select_tuples n g elmt with
-                     | Some tup => set_add str_gt_list_ot.eq_dec tup acc
-                     | None => acc
-                     end)
+  Definition select_relation_f (n: string) (g: ground_types) (elmt: tup_type) (acc: tt_set.t) :=
+    match select_tuples n g elmt with
+    | Some tup => tt_set.add tup acc
+    | None => acc
+    end.
+
+  Arguments select_relation_f _ _ / _ _.
+
+  Definition select_relation (n: string) (g: ground_types) (v: tt_set.t) :=
+    tt_set.fold (select_relation_f n g)
                   v
-                  (@empty_set tup_type).
+                  (tt_set.empty).
+  Arguments select_relation / _ _ _.
 
-  Definition proj_relation (pvs: list string) (v: ListSet.set tup_type) :=
-    set_fold_left (fun (acc: option (ListSet.set tup_type)) (elmt: tup_type) =>
+  Definition proj_relation (pvs: list string) (v: tt_set.t) :=
+    tt_set.fold (fun (elmt: tup_type) (acc: option tt_set.t) =>
                      match proj_tuples pvs elmt with
-                     | Some tup => option_map (set_add str_gt_list_ot.eq_dec tup) acc
+                     | Some tup => option_map (tt_set.add tup) acc
                      | None => None
                      end)
                   v
-                  (Some (@empty_set tup_type)).
+                  (Some (tt_set.empty)).
+
+  Arguments proj_relation / _ _.
 
   Definition assign_vars_to_tuples (R: rel) (v: list (list ground_types)) :=
     List.fold_left (fun acc elmt =>
                       match variable_list_groundings_to_assoc_list R elmt with
-                      | Some l => set_add str_gt_list_ot.eq_dec l acc
+                      | Some l => tt_set.add l acc
                       | None => acc
                       end)
                    v
-                   (@empty_set tup_type).
+                   (tt_set.empty).
+  Arguments assign_vars_to_tuples / _ _.
 
   Print ground_maps.
 
@@ -328,40 +337,40 @@ Module RelSemantics.
   Definition gm_type := ground_maps.t gt_set_type.
 
                         
-  Inductive monotone_op_semantics : gm_type -> monotone_ops -> (ListSet.set tup_type) -> Prop :=
+  Inductive monotone_op_semantics : gm_type -> monotone_ops -> tt_set.t -> Prop :=
   | atom_semantics :
     forall (R: rel) (g: gm_type) (v: list (list ground_types)),
       ground_maps.find (name R) g = Some v ->
       monotone_op_semantics g (ATOM R) (assign_vars_to_tuples R v)
   | select_semantics :
-    forall (g: gm_type) (v v': ListSet.set tup_type) (n: string) (gt: ground_types) (m: monotone_ops),
+    forall (g: gm_type) (v v': tt_set.t) (n: string) (gt: ground_types) (m: monotone_ops),
       monotone_op_semantics g m v ->
       v' = select_relation n gt v ->
       monotone_op_semantics g (SELECT n gt m) v'
   | join_semantics :
     forall (g: gm_type) (m1 m2: monotone_ops)
-      (jvs: list string) (v1 v2 v: (ListSet.set tup_type)),
+      (jvs: list string) (v1 v2 v: (tt_set.t)),
       monotone_op_semantics g m1 v1 ->
       monotone_op_semantics g m2 v2 ->
       v = join_relations jvs v1 v2 ->
       monotone_op_semantics g (JOIN jvs m1 m2) v
   | union_semantics :
     forall (g: gm_type) (m1 m2: monotone_ops)
-      (v1 v2 v: ListSet.set tup_type),
+      (v1 v2 v: tt_set.t),
       monotone_op_semantics g m1 v1 ->
       monotone_op_semantics g m2 v2 ->
-      v = set_union str_gt_list_ot.eq_dec v1 v2 ->
+      v = tt_set.union v1 v2 ->
       monotone_op_semantics g (UNION m1 m2) v
   | proj_semantics :
     forall (g: gm_type) (m: monotone_ops)
-      (pvs: list string) (v v': ListSet.set tup_type),
+      (pvs: list string) (v v': tt_set.t),
       monotone_op_semantics g m v ->
       proj_relation pvs v = Some v' ->
       monotone_op_semantics g (PROJ pvs m) v'.
 
   Fixpoint monotone_op_semantics_eval
            (g: gm_type)
-           (m: monotone_ops) : option (ListSet.set tup_type) :=
+           (m: monotone_ops) : option (tt_set.t) :=
     match m with
     | UNIT => None
     | ATOM R =>
@@ -387,7 +396,7 @@ Module RelSemantics.
         match monotone_op_semantics_eval g m1,
           monotone_op_semantics_eval g m2 with
         | Some v1, Some v2 =>
-            Some (set_union str_gt_list_ot.eq_dec v1 v2)
+            Some (tt_set.union v1 v2)
         | _, _ => None
         end
     | PROJ pvs m =>
@@ -399,7 +408,7 @@ Module RelSemantics.
     end.
 
   Lemma monotone_op_semantics_det :
-    forall (m: monotone_ops) (g: gm_type) (v v': ListSet.set tup_type),
+    forall (m: monotone_ops) (g: gm_type) (v v': tt_set.t),
       monotone_op_semantics g m v ->
       monotone_op_semantics g m v' ->
       v = v'.
@@ -418,7 +427,7 @@ Module RelSemantics.
   Qed.
 
   Lemma monotone_op_semantics_adequacy :
-    forall (m: monotone_ops) (g: gm_type) (v: ListSet.set tup_type),
+    forall (m: monotone_ops) (g: gm_type) (v: tt_set.t),
       Some v = monotone_op_semantics_eval g m <->
         monotone_op_semantics g m v.
   Proof.
@@ -474,12 +483,13 @@ Module RelSemantics.
         * eapply IHm2 in H4. rewrite <- H4 in X0. inversion X0.
       + eapply IHm1 in H2. rewrite <- H2 in X. inversion X.
     - simpl in H. destruct_hyp_match.
-      econstructor. eapply IHm. symmetry. eassumption.
+      econstructor. eapply IHm. symmetry. eassumption. simpl. 
       congruence.
     - simpl. inversion H. subst. destruct_goal_match.
       symmetry in X.
       eapply IHm in X.
       pose proof (monotone_op_semantics_det _ _ _ _ H3 X). subst.
+      simpl in *.
       congruence.
       eapply IHm in H3. rewrite X in H3. congruence.
     - simpl in H. destruct_hyp_match. destruct_hyp_match.
@@ -506,8 +516,8 @@ Module RelSemantics.
 
   Definition anonymize_tuples
              (names: list string)
-             (v: ListSet.set tup_type) : option (list (list ground_types)) :=
-    set_fold_right (fun elmt acc =>
+             (v: tt_set.t) : option (list (list ground_types)) :=
+    tt_set.fold (fun elmt acc =>
                       match anonymize_tuple names elmt with
                       | Some t =>
                           option_map (set_add List_Ground_Type_as_OTF.eq_dec t) acc
@@ -515,6 +525,8 @@ Module RelSemantics.
                       end)
                    v
                    (Some (@empty_set List_Ground_Type_as_OTF.t)).
+
+  Arguments tt_set.fold [A]%type_scope f%function_scope s _ /.
 
   Check ground_maps.mapi.
 
@@ -542,7 +554,7 @@ Module RelSemantics.
       rule_semantics g nil g
   | cons_rules_semantics :
     forall (g g' g'': gm_type)
-      (v: ListSet.set tup_type)
+      (v: tt_set.t)
       (rel_name: string)
       (m: monotone_ops) (R: rel)
       (new_tuples old_tuples: list (list ground_types))
@@ -693,7 +705,7 @@ Module RelSemantics.
      don't have fuel -> fail
 
 
- *)
+   *)
 
   Inductive program_semantics : gm_type -> list (string * rel * monotone_ops) -> gm_type -> Prop :=
   | program_step_done :
@@ -708,16 +720,134 @@ Module RelSemantics.
       program_semantics g' rulez g'' ->
       program_semantics g rulez g''.
 
+
+  Ltac invs H := inversion H; subst.
+  Ltac invc H := inversion H; subst; clear H.
+
+  Lemma tt_set_eq_refl :
+    forall (v v': tt_set.t),
+      v = v' ->
+      tt_set.Equal v v'.
+  Proof.
+    intros. subst. unfold tt_set.Equal. intros; split; intros; eassumption.
+  Qed.
+
+  Print select_relation.
+
+  Print tt_set.Raw.fold.
+  Arguments tt_set.Raw.fold [B]%type_scope f%function_scope _ _ /.
+
+  Lemma tt_set_fold_In_init :
+    forall (v init: tt_set.t) (f: tup_type -> tt_set.t -> tt_set.t),
+      (forall (t: tup_type) (v': tt_set.t),
+          tt_set.Subset v' (f t v')) ->
+      forall init',
+        tt_set.Subset init init' ->
+        tt_set.Subset init (tt_set.fold f v init').
+  Proof.
+    destruct v. rename this0 into v. induction v; intros; simpl.
+    - unfold tt_set.fold. unfold tt_set.Raw.fold. simpl. unfold tt_set.Subset; intros; eauto.
+    - unfold tt_set.fold. unfold tt_set.Raw.fold. simpl.
+      unfold tt_set.fold in IHv. unfold tt_set.Raw.fold in IHv. simpl in IHv.
+      invs is_ok0. specialize (IHv H4). eapply IHv.
+      eassumption.
+      specialize (H a init').
+      unfold tt_set.Subset in *.
+      intros. eapply H. eapply H0. eassumption.
+  Qed.
+
+  Definition monotone (f: tup_type -> tt_set.t -> tt_set.t) :=
+    forall (t: tup_type) (v: tt_set.t),
+      tt_set.Subset v (f t v).
+
+  Arguments monotone f /.
+      
+      
+
+  Lemma tt_set_fold_In :
+    forall (v: tt_set.t) (f: tup_type -> tt_set.t -> tt_set.t) (f': tup_type -> option tup_type) (init: tt_set.t) (t t': tup_type),
+      tt_set.In t v ->
+      f' t = Some t' ->
+      tt_set.In t' (f t init) ->
+      monotone f ->
+      (* (forall (t'': tup_type) (v'': tt_set.t), tt_set.Subset v'' (f t'' v'')) -> *)
+      tt_set.In t' (tt_set.fold f v init).
+  Proof.
+    intros v. destruct v. rename this0 into v. induction v; simpl; intros.
+    - inversion H.
+    - invs is_ok0.
+      specialize (IHv H6).
+      specialize (IHv f f').
+      unfold tt_set.In. unfold tt_set.Raw.In.
+      unfold tt_set.fold. unfold tt_set.Raw.fold. simpl.
+      unfold tt_set.In in IHv. unfold tt_set.Raw.In in IHv. simpl in IHv. unfold tt_set.fold in IHv. unfold tt_set.Raw.fold in IHv. simpl in IHv.
+      invs H.
+      + specialize (H2 t' (Basics.flip f init a)).
+        unfold Basics.flip in H2.
+        unfold tt_set.Subset in H2.
+        pose proof (tt_set_fold_In_init).
+        simpl in H3.
+        unfold tt_set.Subset in H3.
+        admit.
+  Admitted.
+        
+        
+      
+      
+  Lemma tt_set_fold_equal :
+    forall (v v': tt_set.t) (A: Type) (f: tup_type -> tt_set.t -> tt_set.t) (init: tt_set.t),
+      tt_set.Equal v v' ->
+      tt_set.Equal (tt_set.fold f v init) (tt_set.fold f v' init).
+  Proof.
+    intros v. destruct v. induction this0; intros.
+    - unfold tt_set.Equal in H. unfold tt_set.fold. unfold tt_set.Raw.fold. simpl.
+      destruct v'.
+      destruct this0.
+      + simpl. reflexivity.
+      + simpl.
+        specialize (H e).
+        destruct H.
+        assert (tt_set.In e {| tt_set.this := e :: this0; tt_set.is_ok := is_ok1 |}).
+        {
+          unfold tt_set.In. unfold tt_set.Raw.In. econstructor. reflexivity.
+        }
+        eapply H0 in H1. inversion H1.
+    - unfold tt_set.fold. unfold tt_set.Raw.fold. simpl.
+      inversion is_ok0. subst.
+      unfold tt_set.Raw.Ok in is_ok0.
+      specialize (IHthis0 H3).
+      destruct v'. destruct this1.
+      + simpl. unfold tt_set.Equal in H. unfold tt_set.In in H.
+        simpl in H. assert (tt_set.Raw.In a (a :: this0)) by (econstructor; reflexivity).
+        eapply H in H0. inversion H0.
+      + simpl. inversion is_ok1. subst.
+        specialize (IHthis0 {| tt_set.this := this1; tt_set.is_ok := H5 |}).
+        unfold tt_set.fold in IHthis0. unfold tt_set.Raw.fold in IHthis0. simpl in IHthis0.
+        unfold tt_set.Equal.
+        
+        admit.
+  Admitted.
+        
+
+
   Lemma monotone_op_semantics_det' :
-    forall (m: monotone_ops) (g g': gm_type) (v v': ListSet.set tup_type),
+    forall (m: monotone_ops) (g g': gm_type) (v v': tt_set.t),
       ground_maps.Equal g g' ->
       monotone_op_semantics g m v ->
       monotone_op_semantics g' m v' ->
-      (forall x: tup_type,
-          set_mem str_gt_list_ot.eq_dec x v = set_mem str_gt_list_ot.eq_dec x v').
+      tt_set.Equal v v'.
   Proof.
     induction m; unfold ground_maps.Equal; intros.
-    -  
+    - inversion H0.
+    - inversion H0. inversion H1. subst.
+      rewrite H in H4. rewrite H8 in H4. invs H4.
+      eapply tt_set_eq_refl. reflexivity.
+    - invs H0. invs H1. specialize (IHm _ _ _ _ H H7 H8).
+      
+      unfold select_relation.
+      unfold assign_vars_to_tuples in *.
+      admit.
+  Admitted.
     
 
   Lemma rule_semantics_det' :
@@ -730,6 +860,8 @@ Module RelSemantics.
     induction rulez; intros.
     - inversion H0. inversion H1. subst. eassumption.
     - inversion H0. inversion H1. subst. inversion H12; subst; clear H12.
+      admit.
+  Admitted.
       
 
   Lemma program_semantics_det :
@@ -744,6 +876,8 @@ Module RelSemantics.
       + unfold ground_maps.Equal. intros; reflexivity.
       + unfold ground_maps.Equal in *. intros. rewrite H0.
         pose proof (rule_semantics_det _ _ _ _ H H2). subst.
+        admit.
+  Admitted.
         
       
       
